atomic_deduction.v
@@ -22,5 +22,6 @@ Section atomic.
   Lemma translation_subst_atm sigma q : «subst_form sigma (inj q)» = subst_form sigma «inj q».
   Proof. destruct q; repeat now rewrite translation_subst.
   Defined.
-
-End atomic.
+  Lemma translation_subst_atm sigma p : « subst_form_atomic _ _ sigma p » = subst_form sigma (translate_atomic p).
+  Proof. destruct p. cbn. unfold Pred_. rewrite translation_inj. unfold translate_atomic. rewrite subst_dn.
+    rewrite subst_form_inj. reflexivity.
