existential_deduction.v
@@ -39,6 +39,14 @@ Section Existential.
 
 End Existential.
 
+  Variable subst_form_inj : forall sigma p, subst_form sigma (inj p) = subst_form_existential _ subst_form _ sigma p.
+  Variable subst_dn : forall sigma p, subst_form sigma (¬¬p) = ¬¬(subst_form sigma p).
+  Variable translation_subst : forall sigma q, «subst_form sigma q» = subst_form sigma «q».
+  Lemma translation_subst_exst sigma p :  « subst_form_existential _ subst_form _ sigma p » = subst_form sigma (translate_exst p).
+  Proof. destruct p; cbn. unfold Exist_. rewrite translation_inj. cbn. rewrite subst_dn. repeat apply congr_Impl_.
+    rewrite subst_form_inj. cbn. apply congr_Exist_; apply translation_subst. all: reflexivity.
+  Defined.
+
 Section translation.
   Context {Sigma : Signature}.
 
